Dafny/examples/Challenge5/Challenge5SimpleSideEffect.i.dfy
@@ -8,7 +8,7 @@ include "../../AbstractNonInterferenceProof.s.dfy"
 include "./Challenge5Code.s.dfy"
 include "./Challenge5_HelperLemmas.i.dfy"
 
-module challenge5 refines UpdatedAbstractNonInterferenceProof{ 
+module challenge5SideEffects refines UpdatedAbstractNonInterferenceProof{ 
     import opened challenge5Code
     import opened challenge5_helpful_lemmas
     import opened general_instructions_behaviors
@@ -16,10 +16,10 @@ module challenge5 refines UpdatedAbstractNonInterferenceProof{
     import opened memory
     import opened other_operations_i
 
-   
-    predicate preConds(codes:lvm_codes, s:lvm_state, s':lvm_state){
+
+     predicate preConds(codes:lvm_codes, s:lvm_state, s':lvm_state){
         
-        && lvm_require(codes,challenge_prob_5_code_write_encrypted_simple(),s,s')
+        && lvm_require(codes,challenge_prob_5_code_write_encrypted_simple_side_effect(),s,s')
         && codes.lvm_Codes?
         && codes.tl.CNil?
         && ValidState(s)
@@ -33,12 +33,12 @@ module challenge5 refines UpdatedAbstractNonInterferenceProof{
         ensures ValidBehaviorNonTrivial(postB);
         
         // By ensuring !RemovedBehaviors(b), this lemma shows that postB does not contain any 'bad' behavior; ie(encrypt has additonal side effects )
-        ensures !RemovedBehaviors(postB);
+        ensures !RemovedBehaviors(postB); // This proof should fail - this post condition is not maintained
 
     {
         postB := [s];
         
-        var fullCode := challenge_prob_5_code_write_encrypted_simple();
+        var fullCode := challenge_prob_5_code_write_encrypted_simple_side_effect();
         var s' :|  lvm_require(codes, fullCode, s, s');
         
         assert s.ok;
@@ -58,6 +58,7 @@ module challenge5 refines UpdatedAbstractNonInterferenceProof{
         var updatedB:behavior, unwrapedCode:lvm_codes, nextState:state := malloc_(postB, codeBlock, call, Int(0,IntType(8,false)), s');
         assert updatedB[0] == s;
 
+        // assert AllocaStep(s.m,4) == nextState.m;
         assert StateNext(s,nextState);
         assert unwrapedCode == codeBlock.tl;
         assert nextState == bls(updatedB);
@@ -83,42 +84,48 @@ module challenge5 refines UpdatedAbstractNonInterferenceProof{
         var cipherText := D(Ptr(0,0,0,1));
         var call2 := D(Int(0,IntType(1,false)));
 
-       assert unwrapedCode.hd == Ins(CALL(call2,encrypt(call,4,KEY,IV_SIZE,cipherText)));
+       assert unwrapedCode.hd == Ins(CALL(call2,encrypt_side_effects(call,4,KEY,IV_SIZE,cipherText)));
 
         currState := nextState;
         assert ValidBehavior(updatedB); 
-        assert bls(updatedB) == nextState;
         assert |updatedB| == 4;
-
-        updatedB, unwrapedCode, nextState := encrypt_(updatedB, unwrapedCode, call2,call,4,KEY,IV_SIZE,cipherText, s');
+        var oldCode := unwrapedCode;
+        updatedB, unwrapedCode, nextState := encryptSideEffect_(updatedB, unwrapedCode, call2,call,4,KEY,IV_SIZE,cipherText, s');
 
         assert unwrapedCode.hd == Ins(STORE(call2,bytes_written));
         assert ValidBehavior(updatedB); 
-        assert |updatedB| == 5;
+        assert |updatedB| == 7;
+        assert ValidState(bls(updatedB));
+        assert (nextState.ok ==> evalCode_lax(oldCode.hd, currState, nextState));
+        assert  lvm_ensure(oldCode, unwrapedCode, currState, nextState, s');
 
+        assert evalCode_lax(lvm_Block(unwrapedCode), nextState, s');
+
+        // assert evalCode(lvm_Block(unwrapedCode), (bls(updatedB)), s');
         updatedB, unwrapedCode, nextState := lvm_lemma_Store(updatedB, unwrapedCode, r, call2, bytes_written);
         assert ValidBehavior(updatedB); 
-        assert |updatedB| == 6;
+        assert |updatedB| == 8;
         
         var call3 := D(Int(1,IntType(4,false)));
         assert unwrapedCode.hd == Ins(CALL(call3,fwrite(bytes_written,4,1,D(Ptr(0,0,0,1)))));
         
         updatedB, unwrapedCode, nextState := fwrite_(updatedB, unwrapedCode, call3, bytes_written,4,1,D(Ptr(0,0,0,1)),s');
         assert ValidBehavior(updatedB); 
-        assert |updatedB| == 7;
+        assert |updatedB| == 9;
         var cmp := D(Int(0,IntType(1,false)));
 
         assert unwrapedCode.hd == Ins(ICMP(cmp,eq,4,call3,D(Int(0,IntType(4,false)))));
         updatedB, unwrapedCode, nextState := lvm_lemma_Icmp(updatedB, unwrapedCode, s', cmp, eq,4,call3,D(Int(0,IntType(4,false))));
         assert ValidBehavior(updatedB); 
-        assert |updatedB| == 8;
-        //
+        assert |updatedB| == 10;
+        
         assert nextState == s';
         assert unwrapedCode == lvm_CNil(); 
         assert updatedB[0] == s;
         assert updatedB[|updatedB|-1] == s';
         assert BehaviorEvalsCode(codes.hd,updatedB);
-        assert !RemovedBehaviors(updatedB);
+        // assert !RemovedBehaviors(updatedB);
+        
         postB := updatedB;
     }
 
@@ -130,11 +137,11 @@ module challenge5 refines UpdatedAbstractNonInterferenceProof{
              && i <= |b|-2 
              && j > i
              && j < |b|
-             && (forall plainText:operand,size:nat,KEY:operand,IV:operand,cipherText:operand :: evalBlock(encrypt(plainText,size,KEY,IV,cipherText),b[i],b[j]))) 
+             && (forall plainText:operand,size:nat,KEY:operand,IV:operand,cipherText:operand :: evalBlock(encrypt_side_effects(plainText,size,KEY,IV,cipherText),b[i],b[j]))) 
              && !stateFramingMultiValue(b[i],b[j])
     }
 
-
+    
        predicate stateFramingMultiValue(s:state,s':state)
     {
 
@@ -142,6 +149,7 @@ module challenge5 refines UpdatedAbstractNonInterferenceProof{
         var cipherText :| ValidOperand(s,cipherText) && ValidState(s);
         var bytes_written :| ValidOperand(s,bytes_written) && ValidState(s);
         var ops := {OperandContents(s,cipherText),OperandContents(s,bytes_written)};
+
 
         ValidState(s)
         && ValidState(s')
@@ -154,5 +162,8 @@ module challenge5 refines UpdatedAbstractNonInterferenceProof{
             && (forall o:operand :: (o.D? && ValidOperand(s,o) && ValidOperand(s',o) && !(OperandContents(s,o) in ops) ) ==> (OperandContents(s,o) == OperandContents(s',o)))
             && s.m == s'.m)
     }
+
+
+
 
 }
