Dafny/examples/Challenge5/Challenge5_HelperLemmas.i.dfy
@@ -3,6 +3,7 @@ include "../../LLVM/types.dfy"
 include "../../LLVM/control_flow.i.dfy"
 include "./Challenge5Code.s.dfy"
 include "../../LLVM/memory.i.dfy"
+include "../../LLVM/generalInstructionsBehavior.i.dfy"
 
 
 module challenge5_helpful_lemmas{
@@ -11,20 +12,7 @@ module challenge5_helpful_lemmas{
     import opened LLVM_def
     import opened types
     import opened memory
-
-
-
-    predicate stateFraming(s:state,s':state,op:operand)
-    {
-        ValidState(s)
-        && ValidState(s')
-        && ValidOperand(s,op)
-        && ValidOperand(s',op)
-        && s.ok == s'.ok
-        && op.LV? ==> (forall lv :: (lv in s.lvs && lv != op.l) ==> (lv in s'.lvs && s.lvs[lv] == s'.lvs[lv]))//(lv in s'.lv && s.lv[op] == s'.lv[op])
-        && op.GV? ==> (forall gv :: (gv in s.gvs && gv != op.g) ==> (gv in s'.gvs && s.gvs[gv] == s'.gvs[gv]))//(lv in s'.lv && s.lv[op] == s'.lv[op])
-        && s.m == s'.m
-    }
+    import opened general_instructions_behaviors
 
 
 lemma {:axiom} challengeStateAssumptions(s:state)
@@ -47,15 +35,12 @@ lemma malloc_(b:behavior,codes:lvm_codes, ptr:operand,size:Data ,sN:lvm_state)
         requires ValidOperand(bls(b),ptr);
         requires challengeStateAssumptionsPred(bls(b));
 
-        // requires codes == malloc(ptr);
         ensures ValidBehaviorNonTrivial(b');
         ensures StateNext(bls(b),s')
         ensures  lvm_ensure(codes, lvm_bM, bls(b), s', sN);
         ensures |b'| == |b| + 1;
         ensures bls(b') == s';
         ensures forall i :: i >=0 && i < |b| ==> b[i] == b'[i];
-
-        // requires exists s' :: lvm_require(codes,malloc(ptr),s,s');
     {
         var s := bls(b);
         assert malloc(size) == ForeignFunction;
@@ -75,9 +60,8 @@ lemma malloc_(b:behavior,codes:lvm_codes, ptr:operand,size:Data ,sN:lvm_state)
         assert ValidState(lvm_sM);
         assert lvm_sM == s;
         assert codes.tl == lvm_bMs;
-        // lvm_bM := codes.tl;
-        assert evalIns(codes.hd.ins,bls(b),s');
 
+        assert evalIns(codes.hd.ins,bls(b),s');
         assert NextStep(s,s',Step.stutterStep());
         assert MemStateNext(s.m,s'.m,MemStep.stutterStep());
         assert StateNext(s,s');
@@ -95,15 +79,12 @@ lemma malloc_(b:behavior,codes:lvm_codes, ptr:operand,size:Data ,sN:lvm_state)
         requires ValidOperand(bls(b),ptr);
         requires challengeStateAssumptionsPred(bls(b));
 
-        // requires codes == malloc(ptr);
         ensures ValidBehaviorNonTrivial(b');
         ensures StateNext(bls(b),s')
         ensures  lvm_ensure(codes, lvm_bM, bls(b), s', sN);
         ensures |b'| == |b| + 1;
         ensures bls(b') == s';
         ensures forall i :: i >=0 && i < |b| ==> b[i] == b'[i];
-
-        // requires exists s' :: lvm_require(codes,malloc(ptr),s,s');
     {
         var s := bls(b);
         assert encryptEmpty() == ForeignFunction;
@@ -123,7 +104,6 @@ lemma malloc_(b:behavior,codes:lvm_codes, ptr:operand,size:Data ,sN:lvm_state)
         assert ValidState(lvm_sM);
         assert lvm_sM == s;
         assert codes.tl == lvm_bMs;
-        // lvm_bM := codes.tl;
         assert evalIns(codes.hd.ins,bls(b),s');
 
         assert NextStep(s,s',Step.stutterStep());
@@ -142,7 +122,6 @@ lemma malloc_(b:behavior,codes:lvm_codes, ptr:operand,size:Data ,sN:lvm_state)
         requires ValidOperand(bls(b),dst);
         requires challengeStateAssumptionsPred(bls(b));
 
-        // requires codes == malloc(ptr);
         ensures ValidBehaviorNonTrivial(b');
         ensures StateNext(bls(b),s')
         ensures  lvm_ensure(codes, lvm_bM, bls(b), s', sN);
@@ -150,7 +129,6 @@ lemma malloc_(b:behavior,codes:lvm_codes, ptr:operand,size:Data ,sN:lvm_state)
         ensures bls(b') == s';
         ensures forall i :: i >=0 && i < |b| ==> b[i] == b'[i];
 
-        // requires exists s' :: lvm_require(codes,malloc(ptr),s,s');
     {
         var s := bls(b);
         assert encryptEmpty() == ForeignFunction;
@@ -170,7 +148,6 @@ lemma malloc_(b:behavior,codes:lvm_codes, ptr:operand,size:Data ,sN:lvm_state)
         assert ValidState(lvm_sM);
         assert lvm_sM == s;
         assert codes.tl == lvm_bMs;
-        // lvm_bM := codes.tl;
         assert evalIns(codes.hd.ins,bls(b),s');
 
         assert NextStep(s,s',Step.stutterStep());
@@ -190,7 +167,6 @@ lemma encrypt_(b:behavior,codes:lvm_codes, ptr:operand ,plainText:operand,size:n
         requires ValidOperand(bls(b),ptr);
         requires challengeStateAssumptionsPred(bls(b));
 
-        // requires codes == malloc(ptr);
         ensures ValidBehaviorNonTrivial(b');
         ensures StateNext(bls(b),s')
         ensures  lvm_ensure(codes, lvm_bM, bls(b), s', sN);
@@ -198,7 +174,6 @@ lemma encrypt_(b:behavior,codes:lvm_codes, ptr:operand ,plainText:operand,size:n
         ensures bls(b') == s';
         ensures forall i :: i >=0 && i < |b| ==> b[i] == b'[i];
 
-        // requires exists s' :: lvm_require(codes,malloc(ptr),s,s');
     {
         var s := bls(b);
         assert encrypt(plainText,size,KEY,IV,cipherText) == ForeignFunction;
@@ -218,7 +193,6 @@ lemma encrypt_(b:behavior,codes:lvm_codes, ptr:operand ,plainText:operand,size:n
         assert ValidState(lvm_sM);
         assert lvm_sM == s;
         assert codes.tl == lvm_bMs;
-        // lvm_bM := codes.tl;
         assert evalIns(codes.hd.ins,bls(b),s');
 
         assert NextStep(s,s',Step.stutterStep());
@@ -228,54 +202,120 @@ lemma encrypt_(b:behavior,codes:lvm_codes, ptr:operand ,plainText:operand,size:n
         assert ValidBehaviorNonTrivial(b');
     }
 
-
-    // lemma encrypt_side_effects_(b:behavior,codes:lvm_codes, ptr:operand ,plainText:operand,size:nat,KEY:operand,IV:operand,cipherText:operand,sN:lvm_state) 
-    //     returns (b':behavior,lvm_bM:lvm_codes, s':lvm_state)
+    lemma encryptSideEffect_(b:behavior,codes:lvm_codes, ptr:operand ,plainText:operand,size:nat,KEY:operand,IV:operand,cipherText:operand,sN:lvm_state) 
+        returns (b':behavior,lvm_bM:lvm_codes, s':lvm_state)
         
-    //     requires ValidBehaviorNonTrivial(b);
-    //     requires lvm_require(codes, Ins(CALL(ptr,encrypt_side_effects(plainText,size,KEY,IV,cipherText))), bls(b), sN)
-    //     requires ValidState(bls(b));
-    //     requires ValidOperand(bls(b),ptr);
-    //     requires challengeStateAssumptionsPred(bls(b));
-
-    //     // requires codes == malloc(ptr);
-    //     ensures ValidBehaviorNonTrivial(b');
-    //     ensures StateNext(bls(b),s')
-    //     ensures  lvm_ensure(codes, lvm_bM, bls(b), s', sN);
-    //     ensures |b'| == |b| + 1;
-    //     ensures bls(b') == s';
-    //     ensures forall i :: i >=0 && i < |b| ==> b[i] == b'[i];
-
-    //     // requires exists s' :: lvm_require(codes,malloc(ptr),s,s');
-    // {
-    //     var s := bls(b);
-    //     assert encrypt_side_effects(plainText,size,KEY,IV,cipherText) == lvm_Codes(Ins(RET(D(Void))),lvm_CNil())  ;
-    //     assert codes.hd == Ins(CALL(ptr,encrypt_side_effects(plainText,size,KEY,IV,cipherText)));
-    //     assert ValidOperand(s,ptr);
-    //     assert !codes.hd.ins.fnc.CNil?;
-    //     assert ValidInstruction(s, codes.hd.ins);
-
-    //     // assert forall s' :: evalIns(codes.hd.ins,bls(b),s') ==> bls(b) == s';
-    //     s' :| evalIns(codes.hd.ins,bls(b),s');
-    //     lvm_bM := codes.tl;
-
-    //     ghost var lvm_ltmp1, lvm_cM:lvm_code, lvm_ltmp2 := lvm_lemma_block(codes, s, sN);
-    //     var lvm_sM := lvm_ltmp1;
-    //     var lvm_bMs := lvm_ltmp2;
-    //     assert ValidState(s);
-    //     assert ValidState(lvm_sM);
-    //     assert lvm_sM == s;
-    //     assert codes.tl == lvm_bMs;
-    //     // lvm_bM := codes.tl;
-    //     assert evalIns(codes.hd.ins,bls(b),s');
-
-    //     assert NextStep(s,s',Step.stutterStep());
-    //     assert MemStateNext(s.m,s'.m,MemStep.stutterStep());
-    //     assert StateNext(s,s');
-    //     b' := b + [s'];
-    //     assert ValidBehaviorNonTrivial(b');
-    // }
+        requires ValidBehaviorNonTrivial(b);
+        requires lvm_require(codes, Ins(CALL(ptr,encrypt_side_effects(plainText,size,KEY,IV,cipherText))), bls(b), sN)
+        requires ValidState(bls(b));
+        requires ValidOperand(bls(b),ptr);
+        requires challengeStateAssumptionsPred(bls(b));
 
 
+        requires ValidOperand(bls(b),plainText)
+        requires ValidOperand(bls(b),cipherText)
+        requires MemValid(bls(b).m)
+        requires OperandContents(bls(b),plainText).Ptr?
+        requires OperandContents(bls(b),cipherText).Ptr?
+        requires OperandContents(bls(b),plainText).size >= OperandContents(bls(b),cipherText).size;
+        requires validBitWidth(size)
+
+        ensures ValidBehaviorNonTrivial(b');
+        ensures  lvm_ensure(codes, lvm_bM, bls(b), s', sN);
+        ensures |b'| == |b| + 3;
+        ensures bls(b') == s';
+        ensures forall i :: i >=0 && i < |b| ==> b[i] == b'[i];
+    {
+        var s := bls(b);
+        assert codes.hd == Ins(CALL(ptr,encrypt_side_effects(plainText,size,KEY,IV,cipherText)));
+        assert ValidOperand(s,ptr);
+        assert !codes.hd.ins.fnc.CNil?;
+        assert ValidInstruction(s, codes.hd.ins);
+        assert codes.hd.ins.fnc == lvm_Codes(Ins(LLVM_MEMCPY(plainText,cipherText,1,false)),encrypt(plainText,size,KEY,IV,cipherText));   
+                  
+        assert evalIns(codes.hd.ins,s,sN) ==> evalBlock(codes.hd.ins.fnc,s,sN);
+        assert evalCode_lax(lvm_Block(codes), s, sN);
+    
+        lvm_bM := codes.tl;
+
+        ghost var lvm_ltmp1, lvm_cM:lvm_code, lvm_ltmp2 := lvm_lemma_block(codes, s, sN);
+        var lvm_sM := lvm_ltmp1;
+        var lvm_bMs := lvm_ltmp2;
+        assert ValidState(s);
+        assert ValidState(lvm_sM);
+
+        assert codes.tl == lvm_bMs;
+        assert evalIns(Ins(CALL(ptr,encrypt_side_effects(plainText,size,KEY,IV,cipherText))).ins,s,lvm_sM);
+        assert evalBlock(codes.hd.ins.fnc,s,lvm_sM);
+        var sidesB := encrypt_side_effects_behavior(codes.hd.ins.fnc,s,plainText,size,KEY,IV,cipherText,lvm_sM);
+        assert bls(b) == sidesB[0];
+
+        b' := b + sidesB;
+        assert NextStep(bls(b),sidesB[0],Step.stutterStep());
+        assert MemStateNext(bls(b).m,sidesB[0].m,MemStep.stutterStep());
+        assert StateNext(bls(b),sidesB[0]);
+        assert ValidBehaviorNonTrivial(b');
+        assert lvm_sM == bls(b');
+        s' := lvm_sM;
+
+    }
+
+
+
+
+lemma encrypt_side_effects_behavior(codes:lvm_codes, s:lvm_state ,plainText:operand,size:nat,KEY:operand,IV:operand,cipherText:operand,sN:lvm_state) 
+        returns (postB:behavior)
+        
+        requires codes == encrypt_side_effects(plainText,size,KEY,IV,cipherText);
+        requires evalBlock(encrypt_side_effects(plainText,size,KEY,IV,cipherText),s,sN);
+        requires codes.lvm_Codes?
+        requires ValidState(s)
+        
+        requires ValidOperand(s,plainText)
+        requires ValidOperand(s,cipherText)
+        requires MemValid(s.m)
+        requires OperandContents(s,plainText).Ptr?
+        requires OperandContents(s,cipherText).Ptr?
+        requires OperandContents(s,plainText).size >= OperandContents(s,cipherText).size;
+        requires validBitWidth(size)
+
+        ensures ValidBehaviorNonTrivial(postB);
+        ensures BehaviorEvalsCode(codes.hd,postB);
+        ensures |postB| == 3;
+        ensures postB[0] == s;
+        ensures bls(postB) == sN;
+
+
+    {
+        postB := [s];
+        var fullCode := encrypt_side_effects(plainText,size,KEY,IV,cipherText);
+                   
+        var s' := sN;
+        assert s.ok;
+        assert evalBlock(codes, s, s');
+        var codeBlock:lvm_codes := codes;
+        var r:state :| evalCode(codes.hd, s, r) && evalBlock(codes.tl, r, s') ;
+        assert r == s';
+        assert codeBlock.hd == Ins(LLVM_MEMCPY(plainText,cipherText,1,false));
+
+        var updatedB, unwrapedCode, nextState := lvm_lemma_MemCpy(postB, codeBlock, r, plainText, cipherText,1);
+        assert |updatedB| == 2;
+
+        assert StateNext(s,nextState);
+        var currState := nextState;
+        assert unwrapedCode == encrypt(plainText,size,KEY,IV,cipherText);
+        assert ValidBehavior(updatedB); 
+        assert forall s'' :: evalBlock(unwrapedCode,currState,s'') ==> currState == s'';
+        var s'' := currState;
+        updatedB := updatedB + [s''];
+        assert NextStep(currState,s'',Step.stutterStep());
+        assert MemStateNext(currState.m,s''.m,MemStep.stutterStep());
+        assert StateNext(currState,s'');
+        assert ValidBehavior(updatedB); 
+        assert BehaviorEvalsCode(codes.hd,updatedB);
+        assert bls(updatedB) == r;
+        postB := updatedB;
+        assert |updatedB| == 3;
+    }
 
 }
